\text{We are given the formula:}
$$1^3 + 2^3 + \cdots + n^3 = \frac{n^2(n+1)^2}{4}$$

\text{We will prove this by induction.}

\textbf{Base Case:} n = 1
$$1^3 = \frac{1^2(1+1)^2}{4}$$
\text{Using basic math operations:}
$$1 = \frac{4}{4}$$
\text{The base case holds true.}

\textbf{Inductive Hypothesis:}
Assume the formula holds for some \(n = k\), i.e.,
$$1^3 + 2^3 + \cdots + k^3 = \frac{k^2(k+1)^2}{4}$$

\textbf{Inductive Step:}
We need to prove that the formula holds for \(n = k+1\), i.e.,
$$1^3 + 2^3 + \cdots + k^3 + (k+1)^3 = \frac{(k+1)^2(k+2)^2}{4}$$

\text{Start with the inductive hypothesis:}
$$\frac{k^2(k+1)^2}{4} + (k+1)^3 = \frac{(k+1)^2(k+2)^2}{4}$$

\text{Factor the left-hand side:}
$$\frac{k^2(k+1)^2}{4} + (k+1)^3 = \frac{(k+1)^2}{4}(k^2 + 4(k+1))$$

\text{Simplify the expression:}
$$\frac{(k+1)^2}{4}(k^2 + 4k + 4) = \frac{(k+1)^2(k+2)^2}{4}$$

\text{Thus, the inductive step is proven.}

\textbf{Conclusion:} 
By mathematical induction, the formula
$$1^3 + 2^3 + \cdots + n^3 = \frac{n^2(n+1)^2}{4}$$
is true for all positive integers \(n\).
