\text{Given that } P = \{a, b\}

\textbf{Base Case:} 
$$P(0) = \{\emptyset\}$$
\text{Therefore:}
$$2^0 = 1$$

\text{Now, if } x = \{a\}, \text{ the power set is } P(x) = \{\{a\}, \emptyset\}.$$
\text{So the inductive hypothesis is } P(x) = 2^k.

\textbf{Inductive Step:}
Now, create a new set \( y \) which contains all of \( x \) and a new element. Therefore:
$$P(y) = 2^{k+1}$$
\text{We can express this as:}
$$P(y) = 2^k \text{ (with element } b) + 2^k \text{ (without element } b)$$
$$= 2 \cdot 2^k = 2^{k+1}$$
\text{Thus, the inductive step holds.}
