\text{Since } \gcd(a, b) = 1,

1 - ar = bs

\text{If } d \in \mathbb{N} \text{ such that } d \mid a \text{ and } d \mid s. \text{ Then } ar \text{ is a multiple of } d \text{ and } bs \text{ is a multiple of } d. \text{ So } bs + ar = 1. 
\text{ Since } 1 \text{ is not a multiple of } d, \text{ therefore } \gcd(a, s) = 1.

\text{For } \gcd(r, b) = 1, \text{ we have } 1 - bs = ar. 
\text{If } d \in \mathbb{N}, \text{ then } ar + br \text{ is a multiple of } d. 
\text{ Since } 1 \text{ is not a multiple of } d, \text{ we have a contradiction, therefore } \gcd(r, b) = 1.

\text{Therefore, we prove that } \gcd(a, s) = \gcd(r, b) = \gcd(r, s) = 1.
